Formatting fixes, update var names to be more clear

src/Crypto/HKDF/HMAC.dfy
@@ -9,48 +9,45 @@ module {:extern "HMAC"} HMAC {
   datatype {:extern "Digests"} Digests = SHA_256 | SHA_384
 
   // Hash length in octets (bytes), e.g. GetHashLength(SHA_256) ==> 256 bits = 32 bytes ==> n = 32
-  function method GetHashLength(digest: Digests): (n: int)
-    ensures digest == SHA_256 ==> n == 32
-    ensures digest == SHA_384 ==> n == 48
+  function method GetHashLength(digest: Digests): int
   {
-    match digest {
-      case SHA_256 => 32
-      case SHA_384 => 48
-    }
+    match digest
+    case SHA_256 => 32
+    case SHA_384 => 48
   }
 
   class {:extern "HMac"} HMac {
 
     // These functions are used to model the extern state
     // https://github.com/dafny-lang/dafny/wiki/Modeling-External-State-Correctly
-    function {:extern} getKey(): seq<uint8> reads this
-    function {:extern} getDigest(): Digests reads this
-    function {:extern} getInputSoFar(): seq<uint8> reads this
+    function {:extern} GetKey(): seq<uint8> reads this
+    function {:extern} GetDigest(): Digests reads this
+    function {:extern} GetInputSoFar(): seq<uint8> reads this
 
     constructor {:extern} (digest: Digests)
-      ensures this.getDigest() == digest
-      ensures this.getInputSoFar() == []
+      ensures this.GetDigest() == digest
+      ensures this.GetInputSoFar() == []
 
     method {:extern "Init"} Init(key: seq<uint8>)
       modifies this
-      ensures this.getKey() == key;
-      ensures this.getDigest() == old(this.getDigest())
-      ensures this.getInputSoFar() == []
+      ensures this.GetKey() == key;
+      ensures this.GetDigest() == old(this.GetDigest())
+      ensures this.GetInputSoFar() == []
 
     method {:extern "BlockUpdate"} Update(input: seq<uint8>)
-      requires |this.getKey()| > 0
+      requires |this.GetKey()| > 0
       requires |input| < INT32_MAX_LIMIT
       modifies this
-      ensures this.getInputSoFar() == old(this.getInputSoFar()) + input
-      ensures this.getDigest() == old(this.getDigest())
-      ensures this.getKey() == old(this.getKey())
+      ensures this.GetInputSoFar() == old(this.GetInputSoFar()) + input
+      ensures this.GetDigest() == old(this.GetDigest())
+      ensures this.GetKey() == old(this.GetKey())
 
     method {:extern "GetResult"} GetResult() returns (s: seq<uint8>)
-      requires |this.getKey()| > 0
+      requires |this.GetKey()| > 0
       modifies this
-      ensures |s| == GetHashLength(this.getDigest())
-      ensures this.getInputSoFar() == []
-      ensures this.getDigest() == old(this.getDigest())
-      ensures this.getKey() == old(this.getKey())
+      ensures |s| == GetHashLength(this.GetDigest())
+      ensures this.GetInputSoFar() == []
+      ensures this.GetDigest() == old(this.GetDigest())
+      ensures this.GetKey() == old(this.GetKey())
   }
 }
